pushing current bounded verification progress

src/verification/lean/.lake/build/ir/SALT/Intrinsics/RVV.c
@@ -1,6 +1,6 @@
 // Lean compiler output
 // Module: SALT.Intrinsics.RVV
-// Imports: public import Init public import SALT.Basic public import SALT.Params
+// Imports: public import Init public import SALT.Basic
 #include <lean/lean.h>
 #if defined(__clang__)
 #pragma clang diagnostic ignored "-Wunused-parameter"
@@ -23,6 +23,10 @@ LEAN_EXPORT lean_object* lp_SALT_SALT_Intrinsics_RVV_vsext__vf2(lean_object*);
 lean_object* l_List_replicateTR___redArg(lean_object*, lean_object*);
 LEAN_EXPORT lean_object* lp_SALT_SALT_Intrinsics_RVV_vmv__v__x(lean_object*, lean_object*);
 lean_object* l_BitVec_mul(lean_object*, lean_object*, lean_object*);
+LEAN_EXPORT lean_object* lp_SALT_List_mapTR_loop___at___00SALT_Intrinsics_RVV_vmul__vx_spec__0(lean_object*, lean_object*, lean_object*);
+LEAN_EXPORT lean_object* lp_SALT_List_mapTR_loop___at___00SALT_Intrinsics_RVV_vmul__vx_spec__0___boxed(lean_object*, lean_object*, lean_object*);
+LEAN_EXPORT lean_object* lp_SALT_SALT_Intrinsics_RVV_vmul__vx(lean_object*, lean_object*);
+LEAN_EXPORT lean_object* lp_SALT_SALT_Intrinsics_RVV_vmul__vx___boxed(lean_object*, lean_object*);
 lean_object* l_BitVec_add(lean_object*, lean_object*, lean_object*);
 LEAN_EXPORT lean_object* lp_SALT_SALT_Intrinsics_RVV_vmacc__vx___lam__0(lean_object*, lean_object*, lean_object*);
 LEAN_EXPORT lean_object* lp_SALT_SALT_Intrinsics_RVV_vmacc__vx___lam__0___boxed(lean_object*, lean_object*, lean_object*);
@@ -58,11 +62,6 @@ LEAN_EXPORT lean_object* lp_SALT_SALT_Intrinsics_RVV_vmax__vx(lean_object*, lean
 lean_object* lp_SALT_SALT_bvSignedMin(lean_object*, lean_object*, lean_object*);
 LEAN_EXPORT lean_object* lp_SALT_List_mapTR_loop___at___00SALT_Intrinsics_RVV_vmin__vx_spec__0(lean_object*, lean_object*, lean_object*);
 LEAN_EXPORT lean_object* lp_SALT_SALT_Intrinsics_RVV_vmin__vx(lean_object*, lean_object*);
-lean_object* lp_SALT_SALT_clamp(lean_object*, lean_object*, lean_object*, lean_object*);
-LEAN_EXPORT lean_object* lp_SALT_SALT_Intrinsics_RVV_rvvElemFn(lean_object*, lean_object*, lean_object*);
-LEAN_EXPORT lean_object* lp_SALT_SALT_Intrinsics_RVV_rvvElemFn___boxed(lean_object*, lean_object*, lean_object*);
-lean_object* l_List_lengthTR___redArg(lean_object*);
-LEAN_EXPORT lean_object* lp_SALT_SALT_Intrinsics_RVV_rvvPipelineFromIntrinsics(lean_object*, lean_object*, lean_object*);
 LEAN_EXPORT lean_object* lp_SALT_List_mapTR_loop___at___00SALT_Intrinsics_RVV_vwsub__vx_spec__0(lean_object* x_1, lean_object* x_2, lean_object* x_3) {
 _start:
 {
@@ -201,6 +200,85 @@ _start:
 {
 lean_object* x_3; 
 x_3 = l_List_replicateTR___redArg(x_2, x_1);
+return x_3;
+}
+}
+LEAN_EXPORT lean_object* lp_SALT_List_mapTR_loop___at___00SALT_Intrinsics_RVV_vmul__vx_spec__0(lean_object* x_1, lean_object* x_2, lean_object* x_3) {
+_start:
+{
+if (lean_obj_tag(x_2) == 0)
+{
+lean_object* x_4; 
+x_4 = l_List_reverse___redArg(x_3);
+return x_4;
+}
+else
+{
+uint8_t x_5; 
+x_5 = !lean_is_exclusive(x_2);
+if (x_5 == 0)
+{
+lean_object* x_6; lean_object* x_7; lean_object* x_8; lean_object* x_9; 
+x_6 = lean_ctor_get(x_2, 0);
+x_7 = lean_ctor_get(x_2, 1);
+x_8 = lean_unsigned_to_nat(32u);
+x_9 = l_BitVec_mul(x_8, x_6, x_1);
+lean_dec(x_6);
+lean_ctor_set(x_2, 1, x_3);
+lean_ctor_set(x_2, 0, x_9);
+{
+lean_object* _tmp_1 = x_7;
+lean_object* _tmp_2 = x_2;
+x_2 = _tmp_1;
+x_3 = _tmp_2;
+}
+goto _start;
+}
+else
+{
+lean_object* x_11; lean_object* x_12; lean_object* x_13; lean_object* x_14; lean_object* x_15; 
+x_11 = lean_ctor_get(x_2, 0);
+x_12 = lean_ctor_get(x_2, 1);
+lean_inc(x_12);
+lean_inc(x_11);
+lean_dec(x_2);
+x_13 = lean_unsigned_to_nat(32u);
+x_14 = l_BitVec_mul(x_13, x_11, x_1);
+lean_dec(x_11);
+x_15 = lean_alloc_ctor(1, 2, 0);
+lean_ctor_set(x_15, 0, x_14);
+lean_ctor_set(x_15, 1, x_3);
+x_2 = x_12;
+x_3 = x_15;
+goto _start;
+}
+}
+}
+}
+LEAN_EXPORT lean_object* lp_SALT_List_mapTR_loop___at___00SALT_Intrinsics_RVV_vmul__vx_spec__0___boxed(lean_object* x_1, lean_object* x_2, lean_object* x_3) {
+_start:
+{
+lean_object* x_4; 
+x_4 = lp_SALT_List_mapTR_loop___at___00SALT_Intrinsics_RVV_vmul__vx_spec__0(x_1, x_2, x_3);
+lean_dec(x_1);
+return x_4;
+}
+}
+LEAN_EXPORT lean_object* lp_SALT_SALT_Intrinsics_RVV_vmul__vx(lean_object* x_1, lean_object* x_2) {
+_start:
+{
+lean_object* x_3; lean_object* x_4; 
+x_3 = lean_box(0);
+x_4 = lp_SALT_List_mapTR_loop___at___00SALT_Intrinsics_RVV_vmul__vx_spec__0(x_2, x_1, x_3);
+return x_4;
+}
+}
+LEAN_EXPORT lean_object* lp_SALT_SALT_Intrinsics_RVV_vmul__vx___boxed(lean_object* x_1, lean_object* x_2) {
+_start:
+{
+lean_object* x_3; 
+x_3 = lp_SALT_SALT_Intrinsics_RVV_vmul__vx(x_1, x_2);
+lean_dec(x_2);
 return x_3;
 }
 }
@@ -684,92 +762,8 @@ x_4 = lp_SALT_List_mapTR_loop___at___00SALT_Intrinsics_RVV_vmin__vx_spec__0(x_2,
 return x_4;
 }
 }
-LEAN_EXPORT lean_object* lp_SALT_SALT_Intrinsics_RVV_rvvElemFn(lean_object* x_1, lean_object* x_2, lean_object* x_3) {
-_start:
-{
-lean_object* x_4; lean_object* x_5; lean_object* x_6; lean_object* x_7; lean_object* x_8; lean_object* x_9; lean_object* x_10; lean_object* x_11; lean_object* x_12; lean_object* x_13; lean_object* x_14; lean_object* x_15; lean_object* x_16; lean_object* x_17; lean_object* x_18; lean_object* x_19; lean_object* x_20; lean_object* x_21; lean_object* x_22; lean_object* x_23; 
-x_4 = lean_ctor_get(x_1, 0);
-lean_inc(x_4);
-x_5 = lean_ctor_get(x_1, 3);
-lean_inc(x_5);
-x_6 = lean_ctor_get(x_1, 5);
-lean_inc(x_6);
-x_7 = lean_ctor_get(x_1, 6);
-lean_inc(x_7);
-x_8 = lean_ctor_get(x_1, 7);
-lean_inc(x_8);
-x_9 = lean_ctor_get(x_1, 8);
-lean_inc(x_9);
-lean_dec_ref(x_1);
-x_10 = lean_unsigned_to_nat(16u);
-x_11 = lean_unsigned_to_nat(8u);
-x_12 = l_BitVec_signExtend(x_11, x_10, x_3);
-x_13 = l_BitVec_signExtend(x_11, x_10, x_4);
-x_14 = l_BitVec_sub(x_10, x_12, x_13);
-lean_dec(x_13);
-lean_dec(x_12);
-x_15 = lean_unsigned_to_nat(32u);
-x_16 = l_BitVec_signExtend(x_10, x_15, x_14);
-x_17 = l_BitVec_mul(x_15, x_16, x_5);
-lean_dec(x_5);
-lean_dec(x_16);
-x_18 = l_BitVec_add(x_15, x_2, x_17);
-lean_dec(x_17);
-x_19 = lp_SALT_SALT_Intrinsics_RVV_rvvRoundingShiftRight(x_18, x_6);
-lean_dec(x_6);
-x_20 = lp_SALT_SALT_signedClamp(x_15, x_19, x_10);
-x_21 = lp_SALT_SALT_signedSatAdd(x_10, x_20, x_7);
-x_22 = lp_SALT_SALT_signedClamp(x_10, x_21, x_11);
-x_23 = lp_SALT_SALT_clamp(x_11, x_22, x_8, x_9);
-return x_23;
-}
-}
-LEAN_EXPORT lean_object* lp_SALT_SALT_Intrinsics_RVV_rvvElemFn___boxed(lean_object* x_1, lean_object* x_2, lean_object* x_3) {
-_start:
-{
-lean_object* x_4; 
-x_4 = lp_SALT_SALT_Intrinsics_RVV_rvvElemFn(x_1, x_2, x_3);
-lean_dec(x_2);
-return x_4;
-}
-}
-LEAN_EXPORT lean_object* lp_SALT_SALT_Intrinsics_RVV_rvvPipelineFromIntrinsics(lean_object* x_1, lean_object* x_2, lean_object* x_3) {
-_start:
-{
-lean_object* x_4; lean_object* x_5; lean_object* x_6; lean_object* x_7; lean_object* x_8; lean_object* x_9; lean_object* x_10; lean_object* x_11; lean_object* x_12; lean_object* x_13; lean_object* x_14; lean_object* x_15; lean_object* x_16; lean_object* x_17; lean_object* x_18; lean_object* x_19; lean_object* x_20; 
-x_4 = lean_ctor_get(x_1, 0);
-lean_inc(x_4);
-x_5 = lean_ctor_get(x_1, 3);
-lean_inc(x_5);
-x_6 = lean_ctor_get(x_1, 5);
-lean_inc(x_6);
-x_7 = lean_ctor_get(x_1, 6);
-lean_inc(x_7);
-x_8 = lean_ctor_get(x_1, 7);
-lean_inc(x_8);
-x_9 = lean_ctor_get(x_1, 8);
-lean_inc(x_9);
-lean_dec_ref(x_1);
-lean_inc(x_3);
-x_10 = lp_SALT_SALT_Intrinsics_RVV_vwsub__vx(x_3, x_4);
-x_11 = lp_SALT_SALT_Intrinsics_RVV_vsext__vf2(x_10);
-x_12 = l_List_lengthTR___redArg(x_3);
-lean_dec(x_3);
-x_13 = l_List_replicateTR___redArg(x_12, x_2);
-x_14 = lp_SALT_SALT_Intrinsics_RVV_vmacc__vx(x_13, x_5, x_11);
-x_15 = lp_SALT_SALT_Intrinsics_RVV_vssra__vx__rnu(x_14, x_6);
-lean_dec(x_6);
-x_16 = lp_SALT_SALT_Intrinsics_RVV_vnclip__wx__i16(x_15);
-x_17 = lp_SALT_SALT_Intrinsics_RVV_vsadd__vx(x_16, x_7);
-x_18 = lp_SALT_SALT_Intrinsics_RVV_vnclip__wx__i8(x_17);
-x_19 = lp_SALT_SALT_Intrinsics_RVV_vmax__vx(x_18, x_8);
-x_20 = lp_SALT_SALT_Intrinsics_RVV_vmin__vx(x_19, x_9);
-return x_20;
-}
-}
 lean_object* initialize_Init(uint8_t builtin);
 lean_object* initialize_SALT_SALT_Basic(uint8_t builtin);
-lean_object* initialize_SALT_SALT_Params(uint8_t builtin);
 static bool _G_initialized = false;
 LEAN_EXPORT lean_object* initialize_SALT_SALT_Intrinsics_RVV(uint8_t builtin) {
 lean_object * res;
@@ -779,9 +773,6 @@ res = initialize_Init(builtin);
 if (lean_io_result_is_error(res)) return res;
 lean_dec_ref(res);
 res = initialize_SALT_SALT_Basic(builtin);
-if (lean_io_result_is_error(res)) return res;
-lean_dec_ref(res);
-res = initialize_SALT_SALT_Params(builtin);
 if (lean_io_result_is_error(res)) return res;
 lean_dec_ref(res);
 return lean_io_result_mk_ok(lean_box(0));
